updates

paper_meunier_finite.v
@@ -768,15 +768,15 @@ Section test3.
   Context (Apk : forall X , RelIndep O X <-> RelIndep M X).
 
   Lemma extend_pk X: preKernel R M X -> (Non_Mabsorbant R B X) ->
-        exists X', preKernel R M X' /\  X [<= O] X' /\ (exists x', x' \in X' /\ ~ (x' \in X)).
+        exists X', preKernel R M X' /\  X [<= O] X' /\ ~ (X = X').
   Proof. by apply: extend. Qed.
   
-  Definition Rst :=[set Sp | Sp.1 [<= O] Sp.2 /\ (exists x', x' \in Sp.2 /\ ~ (x' \in Sp.1))]%classic.
+  Definition Rst :=[set Sp | Sp.1 [<= O] Sp.2 /\ ~ (Sp.1 = Sp.2)]%classic.
   
   Lemma A0 S: S \in (preKernel R M) `&` (Non_Mabsorbant R B) 
               -> exists S', S' \in (preKernel R M) /\ Rst (S, S').
   Proof.
-    rewrite inE => -[Hpk Hna];move: (extend_pk Hpk Hna) => [S' [/mem_set Hpk' [Hle Hd]]].
+    rewrite inE => -[Hpk Hna];move: (extend_pk Hpk Hna) => [S' [/mem_set Hpk' Hle]].
     by exists S';split;[ | rewrite /Rst /=].
   Qed.
 
@@ -798,10 +798,10 @@ Section test3.
   Qed.
 
   Lemma iic_and_prekernels (h : nat -> (set T)):
-    (iic_fun Rst h) -> (forall n, (h n) \in  (preKernel R M))
+    (iic_fun Rst h) -> (forall n, (h n) \in  (preKernel M O))
     -> exists n p,
         allL Rst (mkseq (fun i => h (n + i+1)) p) (h n) (h n)
-        /\ ((h n)::(mkseq (fun i => h (n + i+1)) p)) [\in] (preKernel R M).
+        /\ ((h n)::(mkseq (fun i => h (n + i+1)) p)) [\in] (preKernel M O).
   Proof.
     move => /iic_to_allL [n [p [_ Hiic]]] Hpk.
     exists n, p. split; first exact.
@@ -809,11 +809,12 @@ Section test3.
   Qed.
   
   Lemma iic_and_prekernels_to_cyclic (h : nat -> (set T)):
-    (iic_fun Rst h) -> (forall n, (h n) \in  (preKernel R M))
+    (iic_fun Rst h) -> (forall n, (h n) \in  (preKernel M O))
     -> exists s, O.+ (s,s).
   Proof.
     move => Hiic Hpk;move: (iic_and_prekernels Hiic Hpk) => [n [p [Ha Hpk']]].
     apply: (@Rcyclic T M O (h n) (mkseq (fun i : nat => h (n + i + 1)) p));last first.
+    by [].
   Admitted.
   
   Lemma choose: (exists h, (iic_fun Rst h) /\ (forall n, (h n) \in  (preKernel R M)))
@@ -1457,12 +1458,12 @@ Section ChampetierExt_Theorem.
                     split;[ |rewrite notin_setE in H3;rewrite inE].
     
     move: (@extend T R B O [:set: S] A2 A6 A7 A8 Hpk H3) 
-        => [S' [Hpre [H7 [x' [H8 H9]]]]].
+        => [S' [Hpre [H7 Hne]]].
     exists [:fin: S'].
     by rewrite prekernelP set_to_finK.
     split;first by  rewrite set_to_finK.
     apply/negP => /eqP Heq.
-    by rewrite Heq set_to_finK in H9.
+    by rewrite Heq set_to_finK in Hne.
   Qed.
   
   Lemma Kernel_ChampetierExt: 
