paper_meunier.v
@@ -480,10 +480,8 @@ Section Paper.
     contra; move => H1 /inP H2. 
     have H3: Non_Mabsorbant R B X. move: H1 => [y H1] H3. exists y. rewrite inE.
     split. by []. rewrite notin_setE in H3. by rewrite inE.
-    move: (extend A2 A6 A7 A8 H2 H3) => [X' [/inP H4 [H5 [x' [H6 H7]]]]].
-    exists X'. by []. split. by [].
-    apply /eqP => /seteqP [H8 H9].
-    by move: H6 => /inP/H8/inP H6.
+    move: (extend A2 A6 A7 A8 H2 H3)  => [X' [/inP H4 [H5 H6]]]. 
+    by exists X';[ | split;[ | apply/eqP;symmetry]].
   Qed.
   
   Implicit Type (S X: set T).
